proof-libs/fstar/core/Alloc.Vec.Into_iter.fsti
@@ -1,0 +1,7 @@
+module Alloc.Vec.Into_iter
+
+val t_IntoIter (t: Type0) (_: unit): Type0
+
+[@@ FStar.Tactics.Typeclasses.tcinstance]
+val into_iter_into_iterator (t: Type0): 
+  Core.Iter.Traits.Collect.t_IntoIterator (t_IntoIter t Alloc.Alloc.t_Global)
