proof-libs/fstar/core/Core.Iter.Adapters.Flatten.fsti
@@ -1,0 +1,3 @@
+module Core.Iter.Adapters.Flatten
+
+val t_FlatMap: Type0 -> Type0 -> Type0 -> Type0
