proof-libs/fstar/core/Core.Iter.Adapters.Rev.fsti
@@ -1,0 +1,3 @@
+module Core.Iter.Adapters.Rev
+
+type t_Rev (t:Type0)
