proof-libs/fstar/core/Core.Iter.Adapters.Take.fsti
@@ -1,0 +1,3 @@
+module Core.Iter.Adapters.Take
+
+val t_Take: Type0 -> Type0
