proof-libs/fstar/core/Core.Iter.Sources.Repeat_with.fsti
@@ -1,0 +1,5 @@
+module Core.Iter.Sources.Repeat_with
+
+val t_RepeatWith: Type0 -> Type0
+
+val repeat_with #t (y: Prims.unit -> t): t_RepeatWith (Prims.unit -> t)
