proof-libs/fstar/core/Core.Iter.fsti
@@ -19,6 +19,16 @@ val iterator_enumerate_all it (i: iterator it)
   : t_all (Core.Iter.Adapters.Enumerate.t_Enumerate it) (usize * i.f_Item)
 val iterator_enumerate_step_by it
   : t_step_by (Core.Iter.Adapters.Enumerate.t_Enumerate it)
+val iterator_enumerate_rev it
+  : t_rev (Core.Iter.Adapters.Enumerate.t_Enumerate it)
+val iterator_enumerate_map it (i: iterator it)
+  : t_map (Core.Iter.Adapters.Enumerate.t_Enumerate it) (usize * i.f_Item)
+val iterator_enumerate_flat_map it (i: iterator it)
+  : t_flat_map (Core.Iter.Adapters.Enumerate.t_Enumerate it) (usize * i.f_Item)
+val iterator_enumerate_zip it
+  : t_zip (Core.Iter.Adapters.Enumerate.t_Enumerate it)
+val iterator_enumerate_take it
+: t_take (Core.Iter.Adapters.Enumerate.t_Enumerate it)
 
 instance iterator_enumerate it {| i: iterator it |}: iterator (Core.Iter.Adapters.Enumerate.t_Enumerate it) = 
   let open Core.Iter.Adapters.Enumerate in
@@ -37,6 +47,11 @@ instance iterator_enumerate it {| i: iterator it |}: iterator (Core.Iter.Adapter
     f_fold      = iterator_enumerate_fold      it i;
     f_enumerate = iterator_enumerate_enumerate it;
     f_step_by   = iterator_enumerate_step_by it;
+    f_rev       = iterator_enumerate_rev it;
+    f_map       = iterator_enumerate_map it i;
+    f_flat_map  = iterator_enumerate_flat_map it i;
+    f_zip       = iterator_enumerate_zip it;
+    f_take      = iterator_enumerate_take it;
     f_all       = iterator_enumerate_all it i;
   }
 
@@ -55,6 +70,16 @@ val iterator_step_by_all it (i: iterator it)
   : t_all (Core.Iter.Adapters.Step_by.t_StepBy it) i.f_Item
 val iterator_step_by_step_by it
   : t_step_by (Core.Iter.Adapters.Step_by.t_StepBy it)
+val iterator_step_by_rev it
+  : t_rev (Core.Iter.Adapters.Step_by.t_StepBy it)
+val iterator_step_by_zip it
+  : t_zip (Core.Iter.Adapters.Step_by.t_StepBy it)
+val iterator_step_by_take it
+  : t_take (Core.Iter.Adapters.Step_by.t_StepBy it)
+val iterator_step_by_map it (i: iterator it)
+  : t_map (Core.Iter.Adapters.Step_by.t_StepBy it) i.f_Item
+val iterator_step_by_flat_map it (i: iterator it)
+  : t_flat_map (Core.Iter.Adapters.Step_by.t_StepBy it) i.f_Item
 
 unfold instance iterator_step_by it {| i: iterator it |}: iterator (Core.Iter.Adapters.Step_by.t_StepBy it) = 
   let open Core.Iter.Adapters.Enumerate in
@@ -65,7 +90,12 @@ unfold instance iterator_step_by it {| i: iterator it |}: iterator (Core.Iter.Ad
     f_fold      = iterator_step_by_fold      it i;
     f_enumerate = iterator_step_by_enumerate it  ;
     f_step_by   = iterator_step_by_step_by   it  ;
+    f_rev       = iterator_step_by_rev       it  ;
     f_all       = iterator_step_by_all       it i;
+    f_zip       = iterator_step_by_zip       it  ;
+    f_take      = iterator_step_by_take      it  ;
+    f_map       = iterator_step_by_map       it i;
+    f_flat_map  = iterator_step_by_flat_map  it i;
   }
 
 (**** Slice *)
@@ -79,7 +109,12 @@ let iterator_slice_contains (t: eqtype): t_contains (t_Slice t) t
 val iterator_slice_fold (t: eqtype): t_fold (t_Slice t) t (iterator_slice_contains t)
 val iterator_slice_enumerate (t: eqtype): t_enumerate (t_Slice t)
 val iterator_slice_step_by (t: eqtype): t_step_by (t_Slice t)
+val iterator_slice_rev (t: eqtype): t_rev (t_Slice t)
 val iterator_slice_all (t: eqtype): t_all (t_Slice t) t
+val iterator_slice_zip (t: eqtype): t_zip (t_Slice t)
+val iterator_slice_take (t: eqtype): t_take (t_Slice t)
+val iterator_slice_map (t: eqtype): t_map (t_Slice t) t
+val iterator_slice_flat_map (t: eqtype): t_flat_map (t_Slice t) t
 
 instance iterator_slice (t: eqtype): iterator (t_Slice t) = {
   f_Item = t;
@@ -89,7 +124,12 @@ instance iterator_slice (t: eqtype): iterator (t_Slice t) = {
   f_fold      = iterator_slice_fold      t;
   f_enumerate = iterator_slice_enumerate t;
   f_step_by   = iterator_slice_step_by   t;
+  f_rev       = iterator_slice_rev       t;
   f_all       = iterator_slice_all       t;
+  f_zip       = iterator_slice_zip       t;
+  f_take      = iterator_slice_take      t;
+  f_map       = iterator_slice_map       t;
+  f_flat_map  = iterator_slice_flat_map  t;
 }
 
 (**** Array *)
@@ -101,7 +141,12 @@ let iterator_array_contains (t: eqtype) len: t_contains (t_Array t len) t
 val iterator_array_fold (t: eqtype) len: t_fold (t_Array t len) t (iterator_array_contains t len)
 val iterator_array_enumerate (t: eqtype) len: t_enumerate (t_Array t len)
 val iterator_array_step_by (t: eqtype) len: t_step_by (t_Array t len)
+val iterator_array_rev (t: eqtype) len: t_rev (t_Array t len)
 val iterator_array_all (t: eqtype) len: t_all (t_Array t len) t
+val iterator_array_zip (t: eqtype) len: t_zip (t_Array t len)
+val iterator_array_take (t: eqtype) len: t_take (t_Array t len)
+val iterator_array_map (t: eqtype) len: t_map (t_Array t len) t
+val iterator_array_flat_map (t: eqtype) len: t_flat_map (t_Array t len) t
 
 instance iterator_array (t: eqtype) len: iterator (t_Array t len) = {
   f_Item = t;
@@ -111,6 +156,141 @@ instance iterator_array (t: eqtype) len: iterator (t_Array t len) = {
   f_fold      = iterator_array_fold      t len;
   f_enumerate = iterator_array_enumerate t len;
   f_step_by   = iterator_array_step_by t len;
+  f_rev       = iterator_array_rev t len;
   f_all       = iterator_array_all t len;
+  f_zip       = iterator_array_zip t len;
+  f_take      = iterator_array_take t len;
+  f_map       = iterator_array_map t len;
+  f_flat_map  = iterator_array_flat_map t len;
 }
 
+(**** Zip *)
+(** This lives in this file for cyclic dependencies reasons. *)
+
+val iterator_zip_contains it (i: iterator it) it2 (i2: iterator it2)
+  : t_contains (Core.Iter.Adapters.Zip.t_Zip it it2) (i.f_Item & i2.f_Item)
+val iterator_zip_fold it (i: iterator it) it2 (i2: iterator it2)
+  : t_fold (Core.Iter.Adapters.Zip.t_Zip it it2) (i.f_Item & i2.f_Item) (iterator_zip_contains it i it2 i2)
+val iterator_zip_next it (i: iterator it) it2 (i2: iterator it2)
+  : t_next (Core.Iter.Adapters.Zip.t_Zip it it2) (i.f_Item & i2.f_Item)
+val iterator_zip_enumerate it it2
+  : t_enumerate (Core.Iter.Adapters.Zip.t_Zip it it2)
+val iterator_zip_all it (i: iterator it) it2 (i2: iterator it2)
+  : t_all (Core.Iter.Adapters.Zip.t_Zip it it2) (i.f_Item & i2.f_Item)
+val iterator_zip_step_by it it2
+  : t_step_by (Core.Iter.Adapters.Zip.t_Zip it it2)
+val iterator_zip_rev it it2
+  : t_rev (Core.Iter.Adapters.Zip.t_Zip it it2)
+val iterator_zip_zip it it2
+  : t_zip (Core.Iter.Adapters.Zip.t_Zip it it2)
+val iterator_zip_take it it2
+  : t_take (Core.Iter.Adapters.Zip.t_Zip it it2)
+val iterator_zip_map it (i: iterator it) it2 (i2: iterator it2)
+  : t_map (Core.Iter.Adapters.Zip.t_Zip it it2) (i.f_Item & i2.f_Item)
+val iterator_zip_flat_map it (i: iterator it) it2 (i2: iterator it2)
+  : t_flat_map (Core.Iter.Adapters.Zip.t_Zip it it2) (i.f_Item & i2.f_Item)
+
+unfold instance iterator_zip it {| i: iterator it |} it2 {| i2: iterator it2 |}
+: iterator (Core.Iter.Adapters.Zip.t_Zip it it2) = 
+  let open Core.Iter.Adapters.Enumerate in
+  {
+    f_Item = i.f_Item & i2.f_Item;
+    f_next      = iterator_zip_next      it i it2 i2;
+    f_contains  = iterator_zip_contains  it i it2 i2;
+    f_fold      = iterator_zip_fold      it i it2 i2;
+    f_enumerate = iterator_zip_enumerate it it2;
+    f_step_by   = iterator_zip_step_by   it it2;
+    f_rev       = iterator_zip_rev       it it2;
+    f_all       = iterator_zip_all       it i it2 i2;
+    f_zip       = iterator_zip_zip       it it2;
+    f_take      = iterator_zip_take      it it2;
+    f_map       = iterator_zip_map       it i it2 i2;
+    f_flat_map  = iterator_zip_flat_map  it i it2 i2;
+  }
+
+(**** Rev *)
+(** This lives in this file for cyclic dependencies reasons. *)
+
+val iterator_rev_contains it (i: iterator it)
+  : t_contains (Core.Iter.Adapters.Rev.t_Rev it) i.f_Item
+val iterator_rev_fold it (i: iterator it)
+  : t_fold (Core.Iter.Adapters.Rev.t_Rev it) i.f_Item (iterator_rev_contains it i)
+val iterator_rev_next it (i: iterator it)
+  : t_next (Core.Iter.Adapters.Rev.t_Rev it) i.f_Item
+val iterator_rev_enumerate it
+  : t_enumerate (Core.Iter.Adapters.Rev.t_Rev it)
+val iterator_rev_all it (i: iterator it)
+  : t_all (Core.Iter.Adapters.Rev.t_Rev it) i.f_Item
+val iterator_rev_step_by it
+  : t_step_by (Core.Iter.Adapters.Rev.t_Rev it)
+val iterator_rev_rev it
+  : t_rev (Core.Iter.Adapters.Rev.t_Rev it)
+val iterator_rev_zip it
+  : t_zip (Core.Iter.Adapters.Rev.t_Rev it)
+val iterator_rev_take it
+  : t_take (Core.Iter.Adapters.Rev.t_Rev it)
+val iterator_rev_map it (i: iterator it)
+  : t_map (Core.Iter.Adapters.Rev.t_Rev it) i.f_Item
+val iterator_rev_flat_map it (i: iterator it)
+  : t_flat_map (Core.Iter.Adapters.Rev.t_Rev it) i.f_Item
+
+unfold instance iterator_rev it {| i: iterator it |}: iterator (Core.Iter.Adapters.Rev.t_Rev it) = 
+  let open Core.Iter.Adapters.Enumerate in
+  {
+    f_Item = i.f_Item;
+    f_next      = iterator_rev_next      it i;
+    f_contains  = iterator_rev_contains  it i;
+    f_fold      = iterator_rev_fold      it i;
+    f_enumerate = iterator_rev_enumerate it  ;
+    f_step_by   = iterator_rev_step_by   it  ;
+    f_rev       = iterator_rev_rev       it  ;
+    f_all       = iterator_rev_all       it i;
+    f_zip       = iterator_rev_zip       it  ;
+    f_take      = iterator_rev_take      it  ;
+    f_map       = iterator_rev_map       it i;
+    f_flat_map  = iterator_rev_flat_map  it i;
+  }
+
+(**** Map *)
+(** This lives in this file for cyclic dependencies reasons. *)
+
+val iterator_map_contains it (i: iterator it) res
+  : t_contains (Core.Iter.Adapters.Map.t_Map it res) res
+val iterator_map_fold it (i: iterator it) res
+  : t_fold (Core.Iter.Adapters.Map.t_Map it res) res (iterator_map_contains it i res)
+val iterator_map_next it (i: iterator it) res
+  : t_next (Core.Iter.Adapters.Map.t_Map it res) res
+val iterator_map_enumerate it res
+  : t_enumerate (Core.Iter.Adapters.Map.t_Map it res)
+val iterator_map_all it (i: iterator it) res
+  : t_all (Core.Iter.Adapters.Map.t_Map it res) res
+val iterator_map_step_by it res
+  : t_step_by (Core.Iter.Adapters.Map.t_Map it res)
+val iterator_map_rev it res
+  : t_rev (Core.Iter.Adapters.Map.t_Map it res)
+val iterator_map_take it res
+  : t_take (Core.Iter.Adapters.Map.t_Map it res)
+val iterator_map_zip it res
+  : t_zip (Core.Iter.Adapters.Map.t_Map it res)
+val iterator_map_map it (i: iterator it) res
+  : t_map (Core.Iter.Adapters.Map.t_Map it res) res
+val iterator_map_flat_map it (i: iterator it) res
+  : t_flat_map (Core.Iter.Adapters.Map.t_Map it res) res
+
+unfold instance iterator_map it {| i: iterator it |} res
+: iterator (Core.Iter.Adapters.Map.t_Map it res) = 
+  let open Core.Iter.Adapters.Enumerate in
+  {
+    f_Item = res;
+    f_next      = iterator_map_next      it i res;
+    f_contains  = iterator_map_contains  it i res;
+    f_fold      = iterator_map_fold      it i res;
+    f_enumerate = iterator_map_enumerate it res;
+    f_step_by   = iterator_map_step_by   it res;
+    f_rev       = iterator_map_rev       it res;
+    f_all       = iterator_map_all       it i res;
+    f_zip       = iterator_map_zip       it res;
+    f_take      = iterator_map_take      it res;
+    f_map       = iterator_map_map       it i res;
+    f_flat_map  = iterator_map_flat_map       it i res;
+  }
