proof-libs/fstar/core/Core.Panicking.fst
@@ -7,9 +7,6 @@ type t_AssertKind = | AssertKind_Eq
 
 let panic (message: string {False}): t_Never
   = match () with
-  
-let assert_failed (k: t_AssertKind) x y (z: Core.Option.t_Option unit {False}): t_Never
-  = match () with
 
 let panic_fmt (fmt: Core.Fmt.t_Arguments {False}): t_Never
   = match () with
